Datalog_Utils.thy
@@ -1,0 +1,9 @@
+theory Datalog_Utils
+  imports "../LTS-formalization/Datalog/Datalog"
+begin
+
+lemma solves_lh_lh_iff: "\<rho> \<Turnstile>\<^sub>c\<^sub>l\<^sub>s Cls p args [] \<longleftrightarrow> \<rho> \<Turnstile>\<^sub>l\<^sub>h (p, args)"
+  unfolding solves_cls_def by auto
+
+
+end
